apart_weakening

ppc/ppc.v
@@ -18,6 +18,46 @@ Definition ids_union_map (f : id -> ids) (a : ids) : ids :=
     set_fold_right ids_union (set_map f a) ids_empty.
 Definition ids_is_empty (a : ids) : Prop := forall x : id, not (ids_In x a).
 Definition ids_disjoint (a b : ids) : Prop := ids_is_empty (ids_inter a b).
+(* Another characterization of set disjointness *)
+Definition ids_disjoint2 (a b : ids) : Prop :=
+  forall x : id, ids_In x a -> not (ids_In x b).
+Definition ids_includes (a b : ids) : Prop :=
+  forall x : id, ids_In x b -> ids_In x a.
+
+Lemma ids_disjoint_implies_ids_disjoint2 :
+    forall A B : ids,
+      ids_disjoint A B -> ids_disjoint2 A B.
+Proof.
+  intros A B hyp.
+  unfold ids_disjoint2.
+  intros x H H2.
+  unfold ids_disjoint, ids_is_empty in hyp.
+  specialize hyp with x.
+  unfold ids_In in hyp.
+  assert (set_In x (ids_inter A B)).
+      apply (set_inter_intro id_eq_dec).
+      assumption. assumption.
+  contradiction.
+Qed.
+
+Lemma ids_disjoint2_implies_ids_disjoint :
+    forall A B : ids,
+      ids_disjoint2 A B -> ids_disjoint A B.
+Proof.
+  intros A B hyp.
+  unfold ids_disjoint, ids_inter, ids_is_empty.
+  intros x H.
+  unfold ids_disjoint2 in hyp.
+  specialize hyp with x.
+  unfold ids_In in H.
+  assert (set_In x A /\ set_In x B) as H_conj.
+      apply (set_inter_elim id_eq_dec).
+      assumption.
+  decompose [and] H_conj.
+  assert (~(set_In x B)).
+      apply hyp. assumption.
+  contradiction.
+Qed.
 
 (* Terms *)
 Inductive term : Type :=
@@ -68,40 +108,124 @@ Definition subst_apply_to_id (s : subst) (x : id) : term :=
   | None      => VarT x
   end.
 
-(* A substitution and a term are *apart* if the bound
-   variables of the term do not occur in the substitution
-*)
+(*
+ * To model application of a substitution to a term, we follow
+ * these steps:
+ *
+ * - First, define the *safe* application of a substitution to
+ *   a term. An application is safe if it can assume that variables
+ *   are renamed apart. (It shall receive a proof of the fact that
+ *   variables are renamed apart).
+ *
+ * - Define alpha-equivalence and renaming in terms of the
+ *   safe substitution.
+ *
+ * - Define the general application of a substitution to a term,
+ *   which composes the safe application with a previous step of
+ *   renaming bound variables in the term, for them to be renamed
+ *   apart.
+ *
+ *)
+
+(*
+ * A substitution and a term are *apart* if the bound
+ * variables of the term do not occur in the substitution
+ * (either in the domain, or as free variables in the
+ * codomain).
+ *
+ *)
 Definition apart (s : subst) (t : term) :=
   ids_disjoint (subst_variables s) (bound_vars t).
 
-Lemma apart_iff_disjoint
-           (A B : ids)
-           (hyp : forall x : id, ids_In x A -> not (ids_In x B))
-           : ids_disjoint A B.
+(*
+ * Given a substitution "s" apart from a given term,
+ * "s" is also apart from a term with less bound variables.
+ *)
+Lemma apart_weakening :
+    forall s : subst,
+    forall t1 t2 : term,
+      ids_includes (bound_vars t1) (bound_vars t2) ->
+      apart s t1 -> apart s t2.
 Proof.
-  intros A B hyp.
-  unfold ids_disjoint, ids_inter, ids_is_empty.
-  intros x H.
-  specialize hyp with x.
-  unfold ids_In in H.
-  assert (set_In x A /\ set_In x B) as H_conj.
-      apply (set_inter_elim id_eq_dec).
+  (* Unfold equivalent disjoint definitions *)
+  intros s t1 t2 incl hyp.
+  unfold apart.
+  unfold apart in hyp.
+  assert (ids_disjoint2 (subst_variables s)
+                        (bound_vars t1))
+         as hyp2.
+      apply ids_disjoint_implies_ids_disjoint2.
       assumption.
-  decompose [and] H_conj.
-  assert (~(set_In x B)).
-      apply hyp. assumption.
+  unfold ids_disjoint2 in hyp2.
+  apply ids_disjoint2_implies_ids_disjoint.
+  unfold ids_disjoint2.
+  unfold ids_includes in incl.
+
+  (* Suppose x is both in the substitution and in BV(t2) *)
+  intros x x_in_s x_in_bv_t2.
+  (* x is in BV(t1) *)
+  assert (ids_In x (bound_vars t1)).
+      specialize incl with x.
+      apply incl.
+      assumption.
+  (* x is not in BV(t1) *)
+  specialize hyp2 with x.
+  assert (~ ids_In x (bound_vars t1)).
+      apply hyp2.
+      assumption.
   contradiction.
 Qed.
 
+Lemma bound_vars_lam_pattern :
+  
+
+(*
+ * Given a substitution apart from "(p ->th a)"
+ * it is also apart from "p" and from "a".
+ *)
 Lemma apart_lam_pattern :
-          forall s : subst,
-          forall p : term, forall th : ids, forall a : term,
-          apart s (LamT p th a) ->
-          apart s p.
+    forall s : subst,
+    forall p : term, forall th : ids, forall a : term,
+      apart s (LamT p th a) ->
+      (apart s p /\ apart s a).
 Proof.
+  (* Unfold equivalent disjoint definitions *)
   intros s p th a h_lam.
   unfold apart.
-  SearchAbout empty_set.
+  unfold apart in h_lam.
+  assert (ids_disjoint2 (subst_variables s)
+                        (bound_vars (LamT p th a)))
+         as h_lam2.
+      apply ids_disjoint_implies_ids_disjoint2.
+      assumption.
+  unfold bound_vars in h_lam2.
+  fold bound_vars in h_lam2.
+  unfold ids_disjoint2 in h_lam2.
+
+  split.
+  (* Apart from "p" *)
+
+      apply ids_disjoint2_implies_ids_disjoint.
+      unfold ids_disjoint2.
+      (* Suppose x is both in the substitution and in BV( p ) *)
+      intros x x_in_s x_in_bvp.
+      (* x is in BV( p ->th a ) *)
+      assert (ids_In x (ids_union
+                           (ids_union (bound_vars p)
+                                      (bound_vars a))
+                           th)).
+          apply set_union_intro1.
+          apply set_union_intro1.
+          assumption.
+      (* x is not in BV( p ->th a ) *)
+      specialize h_lam2 with x.
+      assert (~ ids_In x (ids_union (ids_union (bound_vars p)
+                                               (bound_vars a))
+                                    th)).
+          apply h_lam2.
+          assumption.
+      contradiction.
+Qed.
 
 Fixpoint subst_apply_safe
               (s : subst)
